Refactor effect representation
The previous effect of representation of effects as a type-indexed type
family (Type → Type) was causing universe problems. This is an attempt to solve
this. The new representation is that an effect call is a plain type and then
there is an Effect typeclass that provide a function giving the effect return
value.

For end consumer the main change is that events now only have 2 fields, and the
typing prototype are slightly different.

In the process, the concept of an effect associated exception was scrapped
because not every useful. If needed again one can do:
exc := { call : Eff & eff_ret call → False }.

Candidate traces can now contain a trace that is just a list of effect without a
continuing effect, or a return value.

Common/Effects.v
@@ -1,393 +1,188 @@
-(** This file provide support for handling algebraic effects.
-    It uses UIP *)
+(** This file provide support for handling algebraic effects.*)
 
-Require Export Program.Equality.
-From Equations Require Import Equations.
-Require Import CBase CBool.
+Require Import CBase CBool CDestruct.
 Require Import Options.
 From stdpp Require Import base.
 From stdpp Require Import fin.
 From stdpp Require Import vector.
 
 
+(** * Base effect definitions *)
 
+(** An effect is a type that has an associated function that gives the return
+    type. We fix the universe of all effects because they are fixed anyway by
+    monad universe constraints in stdpp, but then it's easier to debug with a
+    named universe. *)
+Universe e.
+Definition eff := Type@{e}.
+Bind Scope type_scope with eff.
 
+Set Typeclasses Unique Instances.
+(** The effect typeclass, declares a type as an effect and provide [eff_ret],
+    the return type function. *)
+Class Effect (Eff : eff) := eff_ret : Eff → Type@{e}.
+#[export] Hint Mode Effect ! : typeclass_instances.
+Unset Typeclasses Unique Instances.
 
-
-
-(** An effected is a function from Type to Type that take the return type of the
-    effect and give the type of all calls that could return that return type.
-
-    This is voluntarily NOT universe polymorphic. It should probably be Set →
-    Set to be honest. *)
-Definition eff := Type → Type.
 
 (** Generic interface for calling an algebraic effect in a monad *)
-Class MCall (Eff : eff) (M : Type → Type) := mcall : ∀ {A}, Eff A → M A.
-#[global] Arguments mcall {_ _ _ _} _ : assert.
-#[global] Instance: Params (@mcall) 4 := {}.
-#[global] Hint Mode MCall - ! : typeclass_instances.
+Class MCall (Eff : eff) `{Effect Eff} (M : Type → Type) :=
+  mcallM : ∀ call : Eff, M (eff_ret call).
+Arguments mcallM {_ _} _ {_} _ : assert.
+#[export] Instance: Params (@mcallM) 2 := {}.
+#[export] Hint Mode MCall - - ! : typeclass_instances.
 
-(** Call a non returning effect. This is not necessarily a failure, so this
-    doesn't automatically implement MThrow *)
-Definition mcall_noret `{EmptyT T, MBind M, MCall Eff M} (call : Eff T) {A} :
-    M A :=
+
+(** [MCall'] is a type inference hack to be able to call [mcallM] without
+    specifying the monad, otherwise Coq type inference fails to propagate the
+    ambient monad type back. Nobody should implement this typeclass directly. *)
+Class MCall' (Eff : eff) `{Effect Eff} (MEff : Type) (call : Eff) :=
+  mcall : MEff.
+Arguments mcall {_ _ _} _ {_}.
+#[export] Instance: Params (@mcall) 2 := {}.
+#[export] Hint Mode MCall' - - ! ! : typeclass_instances.
+
+Hint Extern 1 (@MCall' ?Eff ?H (?M ?T) ?call) =>
+       notypeclasses refine (@mcallM Eff H M _ call): typeclass_instances.
+
+(** Call a non returning effect. This is not necessarily a failure, so this is
+    not directly linked to [MThrow] *)
+Definition mcall_noret `{MBind M, MCall Eff M} (call : Eff)
+   `{EmptyT (eff_ret call)} {A} : M A :=
   x ← mcall call;
   match emptyT x with end.
 
 
-(** Generic sub-effect judgment, in theory this looks like MCall, but make both
-the same causes universes problems. In addition they need a different Hint Mode
-*)
-Class SubEff (Eff Eff' : eff) := eff_inj : ∀ {A}, Eff A → Eff' A.
-#[global] Arguments eff_inj {_ _ _ _} _ : assert.
-#[global] Instance: Params (@eff_inj) 4 := {}.
-#[global] Hint Mode SubEff ! ! : typeclass_instances.
+(** * Sub-Effects and effect conversion *)
 
-#[global] Instance SubEff_default Eff : SubEff Eff Eff | 100 := λ _ x, x.
+(** Transforming an effect into another effect requires giving a conversion for
+    the return value the other way. [repl_eff] is a type that packages this *)
+Definition repl_eff `{Effect Eff} (call : Eff) Eff' `{Effect Eff'} :=
+  {call' : Eff' & eff_ret call' → eff_ret call}.
+(** Helper constructor for [repl_eff]. Generally f should be the identity
+    function when matching over an event *)
+Definition ReplEff' `{Effect Eff, Effect Eff'} {call : Eff} (call' : Eff')
+  (f : eff_ret call' → eff_ret call) : repl_eff call Eff' :=
+  existT call' f.
+Notation ReplEff call := (ReplEff' call (λ x, x)).
+Definition mcall_repl `{Effect Eff, Effect Eff', MCall Eff' M, FMap M}
+  {call : Eff} (reff : repl_eff call Eff') : M (eff_ret call) :=
+  mcall reff.T1 |$> reff.T2.
 
-(* TODO, this might need to be a Hint Extern *)
-Definition MCall_SubEff {E} `{MCall E' M} `{SubEff E E'} : MCall E M :=
-  λ A e, mcall (eff_inj e : E' A).
+(** Sub-Effect judgment: This provide a canonical effect injection relation.
+    There is no associated proof than this is actually an injection*)
+Class SubEff (Eff Eff': eff) `{Effect Eff, Effect Eff'} :=
+  sub_eff : ∀ call : Eff, repl_eff call Eff'.
+Arguments sub_eff {_ _ _ _ _} _ : assert.
+#[export] Instance: Params (@sub_eff) 5 := {}.
+#[export] Hint Mode SubEff ! ! ! ! : typeclass_instances.
 
-#[export] Hint Extern 5 (MCall ?E ?M) =>
+#[global] Instance SubEff_default Eff `{Effect Eff} : SubEff Eff Eff | 100 :=
+  λ call, ReplEff call.
+
+(** When calling an effect in a monad that support a bigger effect, this will
+    automatically search of a [SubEff] relation to do the adequate effect
+    injection *)
+Definition MCall_SubEff Eff Eff'
+  `{Effect Eff, MCall Eff' M, !SubEff Eff Eff', FMap M} : MCall Eff M :=
+  λ call, mcall_repl (sub_eff call).
+
+#[export] Hint Extern 20 (MCall ?E ?M) =>
   tryif (is_evar E) then fail else class_apply MCall_SubEff
   : typeclass_instances.
 
 
-
-
-(** Scope for effect notation *)
-Declare Scope effect_scope.
-Delimit Scope effect_scope with eff.
-Bind Scope effect_scope with eff.
-Open Scope effect_scope.
-
-
-(** For any effect value, either a value to be returned exists, or the effect is
-    an exception and can be converted to the associated exception type *)
-Module Eff.
-  Section Eff.
-    Context {Eff : eff}.
-
-    (** * Effect equality *)
-    Definition eq {T T'} (call : Eff T) (call' : Eff T') :=
-      existT T call = existT T' call'.
-    Infix "=ₑ" := eq (at level 70, no associativity) : effect_scope.
-
-    Definition conv_call {T T'} (eq : T = T') (call : Eff T) : Eff T' :=
-      eq_rect T Eff call T' eq.
-
-    Definition conv_ret {T T'} (eq : T = T') (ret : T) : T' :=
-      eq_rect T (λ x, x) ret T' eq.
-
-    Definition eq_type {T T'} {call : Eff T} {call' : Eff T'} :
-      call =ₑ call' → T = T' := @eq_sigT_fst _ _ _ _ _ _.
-
-    Definition eq_call {T} {call call': Eff T} :
-      call =ₑ call' → call = call' := inj_pair2 _ _ _ _ _.
-
-    Definition eq_call_rew {T} {call call': Eff T} :
-      call =ₑ call' ↔ call = call'.
-    Proof using. split; [apply eq_call | naive_solver]. Qed.
-
-    Lemma existT_eq_type {a b : sigT Eff} : a = b → a.T1 = b.T1.
-    Proof using. scongruence. Qed.
-
-    Lemma existT_eq_simplify (a : sigT Eff) (c : Eff a.T1) :
-      a = existT _ c → a.T2 = c.
-    Proof using.
-      intro H.
-      destruct a.
-      by dependent destruction H.
-    Qed.
-
-
-    (** * Effect Decision *)
-    Class Decision :=
-      decide_eq T T' (c : Eff T) (c' : Eff T') :: base.Decision (c =ₑ c').
-
-    #[global] Instance eff_decision_sigT `{Decision} : EqDecision (sigT Eff).
-    Proof using. intros [] []. solve_decision. Defined.
-
-    #[global] Instance eff_decision_eff `{Decision} T : EqDecision (Eff T).
-    Proof using.
-      refine (λ x y, dec_if (decide (x =ₑ y))).
-      - by apply eq_call.
-      - naive_solver.
-    Defined.
-
-
-    (** * Effect wellformedness
-
-          An effect is wellformed if we have DecisionT for all type that it
-          could ask as return type. In other words if for all effects we can
-          decide if has an empty return type or not *)
-    Class Wf := wf : ∀ T, Eff T → DecisionT T.
-
-
-    (** * Exception representation.
-
-        The goal of this typeclass is to represent all effects that cannot be
-        returned to as a single exception type
-     *)
-    Class Exc := {
-        exc : Type;
-        exc2eff : exc → sigT Eff;
-        eff2exc : ∀ {T}, Eff T → option exc;
-        exc_wf : ∀ e T call,
-          exc2eff e = existT T call ↔ eff2exc call = Some e;
-        exc_empty : ∀ T (call : Eff T), is_Some (eff2exc call) ↔ (T → False)
-        }.
-    Context {E : Exc}.
-
-
-    Lemma exc_empty_helper `{Inhabited T} P: ¬ P → P ↔ (T → False).
-    Proof using. sfirstorder. Qed.
-
-    Lemma exc_no_return T (call : Eff T) : is_Some (eff2exc call) → T → False.
-    Proof using. by rewrite exc_empty. Qed.
-
-    #[global] Instance exc2eff_inj : Inj (=) (=) (exc2eff).
-    Proof using.
-      intros x y H.
-      destruct (exc2eff x) eqn:Heqn.
-      hfcrush use:exc_wf.
-    Qed.
-
-    Definition exc2call (e : exc) := (exc2eff e).T2.
-
-    Lemma exc2call_wf {T} (c : Eff T) e:
-      eff2exc c = Some e ↔ c =ₑ exc2call e.
-    Proof using.
-      unfold exc2call.
-      unfold eq.
-      rewrite <- sigT_eta.
-      sfirstorder use:exc_wf.
-    Qed.
-
-    Lemma ret_or_exc_exc2call e : eff2exc (exc2call e) = Some e.
-    Proof using.
-      unfold exc2call.
-      rewrite <- exc_wf.
-      rewrite <- sigT_eta.
-      reflexivity.
-    Qed.
-
-    #[global] Instance eff2exc_type_empty e : EmptyT (Eff.exc2eff e).T1.
-    Proof using.
-      unfold EmptyT.
-      rewrite <- exc_empty.
-      eexists.
-      by apply ret_or_exc_exc2call.
-    Qed.
-
-    Lemma exc_type_empty e : (exc2eff e).T1 → False.
-    Proof using.
-      intro T.
-      destruct (exc2eff e) eqn:He.
-      eapply exc_no_return.
-      - rewrite exc_wf in He. naive_solver.
-      - assumption.
-    Qed.
-
-
-  End Eff.
-
-  Infix "=ₑ" := Eff.eq (at level 70, no associativity) : effect_scope.
-  #[global] Hint Mode Exc ! : typeclasses_instances.
-  #[global] Arguments Exc : clear implicits.
-  #[global] Arguments exc _ {_}.
-  #[global] Hint Mode Wf ! : typeclasses_instances.
-  #[global] Arguments Wf : clear implicits.
-  #[global] Hint Mode Decision ! : typeclass_instances.
-  #[global] Arguments Decision : clear implicits.
-  #[global] Arguments decide_eq {_ _ _ _} _ _ : simpl never, assert.
-
-  #[global] Hint Rewrite @ret_or_exc_exc2call : eff.
-
-  Ltac Wf_decisionT_apply T :=
-    match goal with
-    | call : ?Eff T |- _ =>
-        let H := fresh "H" in
-        enough (Wf Eff) as H; first apply (H T call)
-    end.
-  #[global] Hint Extern 5 (DecisionT ?T) =>
-           Wf_decisionT_apply T : typeclass_instances.
-
-  Tactic Notation "simplify_eff_eq" "in" ident(H) :=
-    match type of H with
-    | _ = @existT Type ?Eff ?T ?call =>
-        is_var T;
-        let H' := fresh "H" in
-        pose proof (existT_eq_type H) as H'; cbn in H';
-        subst T;
-        apply (@existT_eq_simplify Eff) in H
-    | @existT Type ?Eff ?T ?call = _ =>
-        is_var T;
-        let H' := fresh "H" in
-        pose proof (existT_eq_type H) as H'; cbn in H';
-        subst T;
-        symmetry in H;
-        apply (@existT_eq_simplify Eff) in H;
-        symmetry in H
-    | @Eff.eq _ ?T _ ?call _ =>
-        is_var T;
-        let H' := fresh "H" in
-        pose proof (Eff.eq_type H) as H';
-        subst T;
-        apply Eff.eq_call in H
-    | @Eff.eq _ _ ?T _ ?call =>
-        is_var T;
-        let H' := fresh "H" in
-        pose proof (Eff.eq_type H) as H';
-        subst T;
-        apply Eff.eq_call in H
-    end.
-
-  Tactic Notation "simplify_eff_eq" :=
-    match goal with
-    | H : Eff.eq _ _ |- _ => simplify_eff_eq in H
-    | H : _ = @existT Type _ _ _ |- _ => simplify_eff_eq in H
-    | H : @existT Type _ _ _ = _ |- _ => simplify_eff_eq in H
-    end.
-
-
-  Section Plus.
-    Context {Eff : eff}.
-    Context {Eff' : eff}.
-
-    Definition plus : eff := λ T, (Eff T + Eff' T)%type.
-
-    #[global] Instance plus_wf `{Wf Eff, Wf Eff'} : Wf plus.
-    Proof using. intros T x. destruct x; naive_solver. Qed.
-
-    #[global] Instance plus_dec `{Decision Eff, Decision Eff'} : Decision plus.
-    Proof using.
-      intros T T' c c'.
-      refine (match c, c' with
-              | inl a, inl b => dec_if (decide (a =ₑ b))
-              | inr a, inr b => dec_if (decide (a =ₑ b))
-              | _, _ => right _
-              end);
-        hauto lq:on simp+:simplify_eff_eq.
-    Defined.
-
-    #[global] Program Instance plus_exc `{Exc Eff, Exc Eff'} : Exc plus :=
-      { exc := exc Eff + exc Eff';
-        exc2eff e := match e return sigT plus with
-                     | inl x => existT _ (inl (exc2eff x).T2)
-                     | inr x => existT _ (inr (exc2eff x).T2)
-                     end;
-        eff2exc _ e := match e with
-                     | inl x => inl <$> eff2exc x
-                     | inr x => inr <$> eff2exc x
-                     end
-      }.
-    Next Obligation.
-      intros. cbn.
-      repeat case_split;
-        (split; intro Heq; [simplify_eff_eq | rewrite fmap_Some in Heq]);
-        sauto q:on dep:on use:exc_wf db:eff.
-    Qed.
-    Next Obligation.
-      intros. cbn.
-      case_split;
-        rewrite fmap_is_Some;
-        rewrite exc_empty;
-        reflexivity.
-    Qed.
-
-    (** Effect injection. Most of the time, the correct version is the left one,
-        so it has a higher priority *)
-    #[global] Instance subeff_plusl `{SubEff E Eff} : SubEff E plus | 10 :=
-      λ _ e, inl (eff_inj e).
-    #[global] Instance subeff_plusr `{SubEff E Eff'} : SubEff E plus | 20 :=
-      λ _ e, inr (eff_inj e).
-  End Plus.
-  #[global] Arguments plus : clear implicits.
-
-End Eff.
-Export (hints, notations, ltac.notations) Eff.
-#[export] Hint Rewrite @Eff.exc2call_wf : eff.
-#[export] Hint Rewrite @Eff.ret_or_exc_exc2call : eff.
-#[export] Hint Rewrite @Eff.eq_call_rew : eff.
-
-Infix "+ₑ" := Eff.plus (at level 50, left associativity) : effect_scope.
-Infix "=ₑ" := Eff.eq (at level 70, no associativity) : effect_scope.
-
-
-Infix "=ₑ" := Eff.eq (at level 70, no associativity) : effect_scope.
-Infix "=ₑ@{ A }" := (@Eff.eq A _ _)
-  (at level 70, only parsing, no associativity) : effect_scope.
-
-
-Notation "(=ₑ)" := Eff.eq (only parsing) : effect_scope.
-Notation "( X =ₑ.)" := (Eff.eq X) (only parsing) : effect_scope.
-Notation "(.=ₑ X )" := (λ Y, Y =ₑ X) (only parsing) : effect_scope.
-Notation "(≠ₑ)" := (λ X Y, ¬X =ₑ Y) (only parsing) : effect_scope.
-Notation "X ≠ₑ Y":= (¬X =ₑ Y) (at level 70, no associativity) : effect_scope.
-Notation "( X ≠ₑ.)" := (λ Y, X ≢ Y) (only parsing) : effect_scope.
-Notation "(.≠ₑ X )" := (λ Y, Y ≢ X) (only parsing) : effect_scope.
-
-Notation "(=ₑ@{ Eff } )" := (@Eff.eq Eff _ _) (only parsing) : effect_scope.
-Notation "(≠ₑ@{ Eff } )" := (λ X Y, ¬X =ₑ@{Eff} Y) (only parsing) : effect_scope.
-Notation "X ≠ₑ@{ Eff } Y":= (¬X =ₑ@{ Eff } Y)
-  (at level 70, only parsing, no associativity) : effect_scope.
-
-(** * Tactics about effects *)
-
-(** A version of [decide_eq] but for [Eff.eq]. Similarly, it expects the effect
-    type (Inductive) to be destroyed before the call *)
-Ltac decide_eff_eq :=
-  lazymatch goal with
-  | |- Decision (?l =ₑ ?r) =>
-      unshelve
-        (decide_fields l r
-           ltac:(unfold Eff.eq; (injection as [=] || intro); by simplify_eq);
-         left; abstract (subst; reflexivity))
-         end.
-
-(** * Generic noreturn type
-
-This is intended to mark explicitly effect that are not returning when defining
-custom effects *)
-
-Definition noreturn : Set := ∅%type.
-
-#[global] Instance emptyT_noreturn : EmptyT noreturn.
-Proof. inversion 1. Qed.
-
-(** * Non determinism effect *)
-
-(** MChoice is the standard non determinism effect, doing a n-wise choice
-    n can be 0 in which case this correspond to a no-behavior execution *)
-Inductive MChoice : eff := ChooseFin (n : nat) : MChoice (fin n).
-
-#[global] Instance MChoice_EffWf : Eff.Wf MChoice.
-Proof. intros T [[]]; tc_solve. Qed.
-
-#[global] Instance MChoice_EffDec : Eff.Decision MChoice.
-Proof. intros ? ? [] []; decide_eff_eq. Defined.
-
-Inductive discard_type := discard_value.
-
-(* Not using unit a exception type to be sure that discard is never confused
-   with failing, as mfail is implemented as mthrow unit *)
-#[global] Program Instance MChoice_EffExc : Eff.Exc MChoice :=
-  { exc := discard_type;
-    exc2eff := λ _, existT _ (ChooseFin 0);
-    eff2exc := λ T c,
-      match c return option discard_type with
-      | ChooseFin 0 => Some discard_value
-      | _ => None
-      end
-  }.
-Solve All Obligations with sauto.
+(** * Effect typeclasses *)
+
+(** ** Effect wellformedness
+
+An effect is wellformed if we have DecisionT for all type that it could ask as
+return type. In other words if for all effects we can decide if has an empty
+return type or not *)
+Class EffWf `{Effect Eff} := eff_wf : ∀ call : Eff, DecisionT (eff_ret call).
+#[global] Arguments EffWf _ {_}.
+#[global] Hint Mode EffWf ! ! : typeclasses_instances.
+#[export] Existing Instance eff_wf.
+
+
+(** ** Effect transportability
+
+An effect is computably transportable if all the return value of the effect are
+transportable, even using an opaque effect equality. This is just implementing
+[CTrans] on [eff_ret] *)
+Class EffCTrans `{Effect Eff} := ctrans_eff : CTrans (eff_ret (Eff := Eff)).
+#[global] Arguments EffCTrans _ {_}.
+#[global] Hint Mode EffCTrans ! ! : typeclasses_instances.
+#[export] Existing Instance ctrans_eff.
+
+Class EffCTransSimpl `{EffCTrans Eff} := ctrans_simpl_eff :
+    CTransSimpl (eff_ret (Eff := Eff)).
+#[global] Arguments EffCTransSimpl _ {_ _}.
+#[global] Hint Mode EffCTransSimpl ! ! ! : typeclasses_instances.
+#[export] Existing Instance ctrans_simpl_eff.
+
+(** * Effect sums
+
+This allows to combine two effects in a single effect, mainly to instantiate
+objects like free monads *)
+
+Section Plus.
+  Context Eff `{Effect Eff} Eff' `{Effect Eff'}.
+  #[export] Instance Effect_sum : Effect (Eff + Eff') :=
+    λ call, match call with
+            | inl calll => eff_ret calll
+            | inr callr => eff_ret callr
+            end.
+
+  #[export] Instance EffWf_sum `{!EffWf Eff} `{!EffWf Eff'}: EffWf (Eff + Eff').
+  Proof. intros []; cbn; tc_solve. Defined.
+
+  #[export] Instance EffCTrans_sum `{!EffCTrans Eff} `{!EffCTrans Eff'} :
+    EffCTrans (Eff + Eff').
+  Proof. intros [] [] eq er; cbn in *.
+         all: try abstract discriminate.
+         all: eapply ctrans;[|eassumption].
+         all: abstract naive_solver.
+  Defined.
+
+  #[export] Instance SubEff_suml : SubEff Eff (Eff + Eff') | 100 :=
+    λ x, ReplEff (inl x).
+
+  #[export] Instance SubEff_sumr : SubEff Eff' (Eff + Eff') | 100 :=
+    λ x, ReplEff (inr x).
+End Plus.
+
+
+(** * Non determinism effect: [MChoice] *)
+
+(** MChoice is the standard non determinism effect.
+    [ChooseFin n] is doing a [n]-wise choice.
+    [n] can be 0 in which case this correspond to a no-behavior execution *)
+Inductive MChoice : eff := ChooseFin (n : nat).
+#[export] Instance MChoice_ret : Effect MChoice := λ '(ChooseFin n), fin n.
+
+#[export] Instance MChoice_EffWf : EffWf MChoice.
+Proof. intros []. cbn. tc_solve. Defined.
+
+#[export] Instance MChoice_EffCTrans : EffCTrans MChoice.
+Proof.
+  intros [] [] eq er.
+  cbn in *.
+  eapply ctrans; [|eassumption].
+  abstract (naive_solver).
+Defined.
+
+#[export] Instance MChoice_EffCTransSimpl : EffCTransSimpl MChoice.
+Proof. intros [] ? ?. cbn. by simp ctrans. Qed.
+
+#[export] Instance MChoice_eq_dec : EqDecision MChoice.
+Proof. solve_decision. Defined.
+
+(** ** [MChoice] helper functions *)
 
 (** Special case of MCall for MChoice *)
-Notation MChoose := (MCall MChoice).
-Definition mchoose `{MChoose M} (n : nat) : M (fin n) := mcall (ChooseFin n).
+Notation MChoose := (@MCall MChoice MChoice_ret).
+Definition mchoose `{!MChoose M} (n : nat) : M (fin n) := mcall (ChooseFin n).
 Definition mdiscard `{MChoose M, FMap M} {A} : M A :=
   mcall (ChooseFin 0) |$> (λ x, match (x : fin 0) with end).
 
@@ -408,41 +203,72 @@ Tactic Notation "case_guard_discard" "as" ident(Hx) :=
   match goal with
   | H : context C [@guard_discard ?M ?C ?F ?R ?P ?dec] |- _ =>
       change (@guard_discard M C F R P dec) with (
-        match @decide P dec with left H' => @mret M R P H' | _ => @mdiscard M C F P end) in *;
+        match @decide P dec with
+          left H' => @mret M R P H' | _ => @mdiscard M C F P end) in *;
       destruct_decide (@decide P dec) as Hx
 
   | |- context C [@guard_discard ?M ?C ?F ?R ?P ?dec] =>
       change (@guard_discard M C F R P dec) with (
-        match @decide P dec with left H' => @mret M R P H' | _ => @mdiscard M C F P end) in *;
+        match @decide P dec with
+          left H' => @mret M R P H' | _ => @mdiscard M C F P end) in *;
       destruct_decide (@decide P dec) as Hx
   end.
 Tactic Notation "case_guard_discard" :=
   let H := fresh in case_guard_discard as H.
 
 
-(** * State effect *)
-Inductive MState {St : Type} : eff :=
-| MSet (val : St) : MState unit
-| MGet : MState St.
+(** * State effect: [MState] *)
+
+(** This is the standard state effect with a getter and a setter. The state must
+    be in or below the effect universe *)
+Inductive MState {St : Type@{e}} : eff :=
+| MSet (val : St) : MState
+| MGet : MState.
 Arguments MState : clear implicits.
 
-#[global] Instance MState_EffWf `{Inhabited St} : Eff.Wf (MState St).
-Proof. intros _ []; tc_solve. Qed.
+#[export] Instance MState_ret St : Effect (MState St) :=
+  λ call, match call with
+          | MSet _ => unit
+          | MGet => St
+          end.
 
-#[global] Instance MState_EffDec `{EqDecision St} : Eff.Decision (MState St).
-Proof. intros ? ? [] []; decide_eff_eq. Defined.
+#[export] Instance MState_EffWf `{Inhabited St} : EffWf (MState St).
+Proof. intros []; cbn; tc_solve. Defined.
+
+#[export] Instance MState_EffCTrans St : EffCTrans (MState St).
+Proof.
+  intros [] [].
+  all: try (abstract discriminate).
+  all: cbn in *.
+  all: intros; assumption.
+Defined.
+
+#[export] Instance MState_EffCTransSimpl St : EffCTransSimpl (MState St).
+Proof. by intros [] ? ?. Qed.
+
+#[export] Instance MState_eq_dec `{EqDecision St} : EqDecision (MState St).
+Proof. solve_decision. Defined.
+
+(** ** [MState] helper functions
+
+- [mGet] : get the whole state
+- [mget field] : get the field [field] of the state
+- [mSet upd] : update the state with the function [upd]
+- [mSetv val] : update the state with the value [val]
+- [mset field upd] : update the state field [field] with the function [upd]
+- [msetv field val] : update the state field [field] with the value [val] *)
 
 Notation mGet := (mcall MGet).
-Definition mget `{MCall (MState St) M, FMap M} {T} (proj : St → T) : M T :=
+Definition mget `{!MCall (MState St) M, FMap M} {T} (proj : St → T) : M T :=
   mGet |$> proj.
 
 Notation mSetv s := (mcall (MSet s)).
-Definition mSet `{MCall (MState St) M, MBind M} (upd : St → St) : M unit :=
+Definition mSet `{!MCall (MState St) M, MBind M} (upd : St → St) : M unit :=
   s ← mGet;
   mSetv (upd s).
-Definition mset `{MCall (MState St) M, MBind M} {T} (proj : St → T)
+Definition mset `{!MCall (MState St) M, MBind M} {T} (proj : St → T)
   `{Setter St T proj} (upd : T → T) : M unit :=
   mSet (set proj upd).
-Definition msetv `{MCall (MState St) M, MBind M} {T} (proj : St → T)
+Definition msetv `{!MCall (MState St) M, MBind M} {T} (proj : St → T)
   `{Setter St T proj} (val : T) : M unit :=
   mset proj (λ _, val).
